\documentclass{article}

%other packages
\usepackage[a4paper, total={7.5in, 10.5in}]{geometry}
\usepackage{longtable}
\usepackage{wrapfig}
\setlength\parindent{0pt}
\usepackage{enumitem}
\usepackage[table]{xcolor}
\usepackage{polynom}
\def\scaleint#1{\vcenter{\hbox{\scaleto[3ex]{\displaystyle\int}{#1}}}}
\usepackage{euler}

%maths
\usepackage{mathtools}
\usepackage{amsmath}
\usepackage{amssymb}
\usepackage{amsfonts}
\usepackage{autobreak}

%tikzpicture
\usepackage{tikz}
\usepackage{scalerel}
\usepackage{pict2e}
\usepackage{tkz-euclide}
\usepackage{tikz-3dplot}
\usetikzlibrary{calc}
\usetikzlibrary{patterns,arrows.meta}
\usetikzlibrary{shadows}
\usetikzlibrary{external}

%pgfplots
\usepackage{pgfplots}
\pgfplotsset{compat=newest}
\usepgfplotslibrary{statistics}
\usepgfplotslibrary{fillbetween}

\pgfplotsset{
    standard/.style={
    axis line style = thick,
    trig format=rad,
    enlargelimits,
    axis x line=middle,
    axis y line=middle,
    enlarge x limits=0.15,
    enlarge y limits=0.15,
    every axis x label/.style={at={(current axis.right of origin)},anchor=north west},
    every axis y label/.style={at={(current axis.above origin)},anchor=south east}
    }
}

\begin{document}
\begin{enumerate}[label={\bf{}\arabic*}.]

\item%1
	\begin{align*}
	\int\frac{1}{x^2\sqrt{x^2-9}}\ dx&\overset{x=3\sec\theta}{\underset{dx=3\sec\theta\tan\theta\ d\theta}{=\joinrel=\joinrel=\joinrel=\joinrel=\joinrel=\joinrel=\joinrel=\joinrel=\joinrel=\joinrel=}}\int\frac{1}{3^3\sec^2\theta\cdot3\tan\theta}\cdot3\sec\theta\tan\theta\ d\theta\\
	&=\frac{1}{9}\int\cos\theta\ d\theta\\
	&=\frac{1}{9}\sin\theta+C
	\end{align*}

\item%2
	\begin{align*}
	\int x^3\sqrt{9-x^2}\ dx&\overset{x=3\sin\theta}{\underset{dx=3\cos\theta\ d\theta}{=\joinrel=\joinrel=\joinrel=\joinrel=\joinrel=\joinrel=\joinrel=}}\int3^3\sin^3\theta\cdot3\cos\theta\cdot3\cos\theta\ d\theta\\
	&=3^5\int\sin^3\theta\cos^2\theta\ d\theta\\
	&=3^5\int\sin\theta(\cos^2\theta-\cos^4\theta)\ d\theta\\
	&\overset{u=\cos\theta}{\underset{du=-\sin\theta\ d\theta}{=\joinrel=\joinrel=\joinrel=\joinrel=\joinrel=\joinrel=\joinrel=}}-3^5\int\cos^2\theta-\cos^4\theta\ d\theta\\
	&=-3^5\int\frac{1}{2}(1+\cos(2\theta))-(1+2\cos(2\theta))^2\ d\theta\\
	&=-3^3\int\frac{1}{2}+\cos(2\theta)-1-2\cos(2\theta)-\cos^2(2\theta)\ d\theta\\
	&=-3^5\int-\frac{1}{2}-\cos(2\theta)-\frac{1}{2}-\frac{1}{2}\cos(4\theta)\ d\theta\\
	&=3^5\int1+\cos(2\theta)+\frac{1}{2}\cos(4\theta)\ d\theta\\
	&=3^5\theta+\frac{3^5}{2}\sin(2\theta)+\frac{3^5}{8}\sin(4\theta)+C
	\end{align*}

\color{red}\item[\refstepcounter{enumi}\fbox{\number\value{enumi}.}]\color{black}%3
	\begin{align*}
	\int\frac{x^3}{\sqrt{x^2+9}}\ dx&\overset{x=3\tan\theta}{\underset{dx=3\sec^2\theta\ d\theta}{=\joinrel=\joinrel=\joinrel=\joinrel=\joinrel=\joinrel=\joinrel=}}\int\frac{3^3\tan^3\theta}{3\sec\theta}\cdot3\sec^2\theta\ d\theta\\
	&=3^3\int\tan^3\theta\sec\theta\ d\theta\\
	&=3^3\int\sec\theta\tan\theta\sec^2\theta+\sec\theta\tan\theta\ d\theta\\
	&\overset{u=\sec\theta}{\underset{\sec\theta\tan\theta\ d\theta}{=\joinrel=\joinrel=\joinrel=\joinrel=\joinrel=\joinrel=}}3^3\int u^2+1\ du\\
	&=9u^3+27u+C
	\end{align*}

\item%4
	\begin{align*}
	\int_0^{2\sqrt{3}}\frac{x^3}{\sqrt{16-x^2}}\ dx&\overset{x=4\sin\theta}{\underset{dx=4\cos\theta\ d\theta}{=\joinrel=\joinrel=\joinrel=\joinrel=\joinrel=\joinrel=\joinrel=}}\int_0^\frac{\pi}{3}\frac{4^3\sin^3\theta}{4\cos\theta}\cdot4\cos\theta\ d\theta\\
	&=4^3\int_0^\frac{\pi}{3}\sin\theta(1-\cos^2\theta)\ d\theta\\
	&=4^3\int_0^\frac{\pi}{3}\sin\theta\ d\theta+4^3\int_0^\frac{\pi}{3}-\sin\theta\cos^2\theta\ d\theta\\
	&\overset{u=\cos\theta}{\underset{du=-\sin\theta\ d\theta}{=\joinrel=\joinrel=\joinrel=\joinrel=\joinrel=\joinrel=\joinrel=}}-4^3[\cos\theta]_0^\frac{\pi}{3}+4^3\int_1^\frac{1}{2}u^2\ du\\
	&=2^5+\frac{2^6}{3}u^3\Big|_1^\frac{1}{2}\\
	&=\frac{40}{3}
	\end{align*}

\item%5
	\begin{align*}
    \int_{\sqrt{2}}^2\frac{1}{t^3\sqrt{t^2-1}}\ dt &\overset{t=\sec\theta}{\underset{dt=\sec\theta\tan\theta\ d\theta}{=\joinrel=\joinrel=\joinrel=\joinrel=\joinrel=\joinrel=\joinrel=\joinrel=\joinrel=}}\int_\frac{\pi}{4}^\frac{\pi}{3}\frac{1}{\sec^3\theta\tan\theta}\cdot\sec\theta\tan\theta\ d\theta\\
	&=\int_\frac{\pi}{4}^\frac{\pi}{3}\cos^2\theta\ d\theta\\
	&=\int_\frac{\pi}{4}^\frac{\pi}{3}1+\cos(2\theta)\ d\theta\\
	&=\theta+\frac{1}{2}\sin(2\theta)\Big|_\frac{\pi}{4}^\frac{\pi}{3}\\
	&=[(\frac{\pi}{3}+\frac{1}{2}\cdot\frac{\sqrt{3}}{2})-(\frac{\pi}{4}+\frac{1}{2}\cdot1)]\\
	&=\frac{\pi+3\sqrt{3}-6}{12}
	\end{align*}

\item%6
	\begin{align*}
	\int_1^2\frac{\sqrt{x^2-1}}{x}\ dx&\overset{x=\sec\theta}{\underset{dx=\sec\theta\tan\theta\ d\theta}{=\joinrel=\joinrel=\joinrel=\joinrel=\joinrel=\joinrel=\joinrel=\joinrel=\joinrel=}}\int_0^\frac{\pi}{3}\tan^2\theta\ d\theta\\
	&=\int_0^\frac{\pi}{3}\sec^2\theta-1\ d\theta\\
	&=\tan\theta-\theta\Big|_0^\frac{\pi}{3}\\
	&=\sqrt{3}-\frac{\pi}{3}
	\end{align*}

\color{red}\item[\refstepcounter{enumi}\fbox{\number\value{enumi}.}]\color{black}%7
	\begin{align*}
	\int\frac{1}{x^2\sqrt{25-x^2}}\ dx&\overset{x=5\sin\theta}{\underset{dx=5\cos\theta\ d\theta}{=\joinrel=\joinrel=\joinrel=\joinrel=\joinrel=\joinrel=\joinrel=}}\int\frac{1}{25\sin\theta\cdot5\cos\theta}\cdot5\cos\theta\ d\theta\\
	&=\frac{1}{25}\int\sec\theta\ d\theta\\
	&=\frac{1}{25}\int\frac{\sec^2\theta+\sec\theta\tan\theta}{\sec\theta+\tan\theta}\ d\theta\\
	&\overset{u=\sec\theta+\tan\theta}{\underset{du=\sec\theta\tan\theta+\sec^2\theta\ d\theta}{=\joinrel=\joinrel=\joinrel=\joinrel=\joinrel=\joinrel=\joinrel=\joinrel=\joinrel=\joinrel=\joinrel=\joinrel=\joinrel=}}\frac{1}{25}\int\frac{1}{u}\ du\\
	&=\frac{1}{25}\ln|\sec\theta+\tan\theta|+C
	\end{align*}

\item%8
	\begin{align*}
	\int\frac{x^3}{\sqrt{x^2+100}}\ dx&\overset{x=10\tan\theta}{\underset{dx=10\sec^2\theta\ d\theta}{=\joinrel=\joinrel=\joinrel=\joinrel=\joinrel=\joinrel=\joinrel=\joinrel=}}100\int\cos\theta\ d\theta\\
	&=100\sin\theta+C
	\end{align*}

\item%9
	\begin{align*}
	\int\frac{dx}{\sqrt{x^2+16}}&\overset{x=4\tan\theta}{\underset{dx=4\sec^2\theta\ d\theta}{=\joinrel=\joinrel=\joinrel=\joinrel=\joinrel=\joinrel=\joinrel=}}\frac{1}{4}\int\cos\theta\ d\theta\\
	&=\frac{1}{4}\sin\theta+C
	\end{align*}

\item%10
	\begin{align*}
	\int\frac{t^5}{\sqrt{t^2+2}}\ dt&\overset{t=\sqrt{2}\tan\theta}{\underset{dt=\sqrt{2}\sec^2\theta\ d\theta}{=\joinrel=\joinrel=\joinrel=\joinrel=\joinrel=\joinrel=\joinrel=\joinrel=}}\int\frac{2^\frac{5}{2}\tan^5\theta}{\sqrt{2}\sec\theta}\cdot\sqrt{2}\sec^2\theta\ d\theta\\
	&=2^\frac{5}{2}\int\sin^5\theta\cos^4\theta\ d\theta\\
	&=2^\frac{5}{2}\int\sin\theta(1-\cos^2\theta)^2\cos^4\theta\ d\theta\\
	&=2^\frac{5}{2}\int\sin\theta(1-\cos^2\theta)(\cos^4\theta-\cos^6\theta)\ d\theta\\
	&=-2^\frac{5}{2}\int-\sin\theta(\cos^4\theta-2\cos^6\theta+\cos^8\theta)\ d\theta\\
	&\overset{u=\cos\theta}{\underset{du=-\sin\theta\ d\theta}{=\joinrel=\joinrel=\joinrel=\joinrel=\joinrel=\joinrel=\joinrel=}}-2^\frac{5}{2}\int u^4-2u^6+u^8\ du\\
	&=-2^\frac{5}{2}[\frac{u^5}{5}-2\frac{u^7}{7}+\frac{u^9}{9}]+C
	\end{align*}

\item%11
	\begin{align*}
	\int\sqrt{1-4x^2}\ dx&\overset{u=2x}{\underset{du=2\ dx}{=\joinrel=\joinrel=\joinrel=\joinrel=}}\frac{1}{2}\int\sqrt{1-u^2}\ du\\
	&\overset{u=\sin\theta}{\underset{du=\cos\theta\ d\theta}{=\joinrel=\joinrel=\joinrel=\joinrel=\joinrel=\joinrel=}}\frac{1}{2}\int\cos^2\theta\ d\theta\\
	&=\frac{1}{4}\int1+\cos(2\theta)\ d\theta\\
	&=\frac{1}{4}[\theta+\frac{1}{2}\sin(2\theta)]+C
	\end{align*}

\item%12
	\begin{align*}
	\int_0^1x\sqrt{x^2+4}\ dx&\overset{x=2\tan\theta}{\underset{dx=2\sec^2\theta\ d\theta}{=\joinrel=\joinrel=\joinrel=\joinrel=\joinrel=\joinrel=\joinrel=\joinrel=}}8\int_0^{\arctan\frac{1}{2}}\tan\theta\sec^3\theta\ d\theta\\
	&\overset{u=\sec\theta}{\underset{du=\sec\theta\tan\theta\ d\theta}{=\joinrel=\joinrel=\joinrel=\joinrel=\joinrel=\joinrel=\joinrel=\joinrel=\joinrel=}}8\int_1^{\sec(\arctan\frac{1}{2})}u^2\ du\\
	&=\frac{8}{3}u^3\Big]_1^{\sec(\arctan\frac{1}{2})}\Big|_{u=\sec\theta}\\
	&=\frac{8}{3}\sec^3\theta\Big]_0^{\arctan\frac{1}{2}}\\
	&=\frac{8}{3}(1+\tan^2\theta)^\frac{3}{2}\Big]_0^{\arctan\frac{1}{2}}\Big|_{\theta=\arctan\frac{x}{2}}\\
	&=\frac{8}{3}(1+\tan^2(\arctan\frac{x}{2}))^\frac{3}{2}\Big]_0^1\\
	&=\frac{8}{3}(1+\frac{x^2}{4})^\frac{3}{2}\Big]_0^1\\
	&=\frac{5\sqrt{5}-8}{3}
	\end{align*}

\color{red}\item[\refstepcounter{enumi}\fbox{\number\value{enumi}.}]\color{black}%13
	\begin{align*}
	\int\frac{\sqrt{x^2-9}}{x^3}\ dx&\overset{x=3\sec\theta}{\underset{dx=3\sec\theta\tan\theta\ d\theta}{=\joinrel=\joinrel=\joinrel=\joinrel=\joinrel=\joinrel=\joinrel=\joinrel=\joinrel=\joinrel=}}\frac{1}{3}\int\sin^2\theta\\
	&=\frac{1}{3}\int1-\cos(2\theta)\ d\theta\\
	&=\frac{\theta}{3}-\frac{1}{6}\sin(2\theta)+C
	\end{align*}

\item%14
	\begin{align*}
	\int\frac{du}{u\sqrt{5-u^2}}&\overset{u=\sqrt{5}\sin\theta}{\underset{du=\sqrt{5}\cos\theta\ d\theta}{=\joinrel=\joinrel=\joinrel=\joinrel=\joinrel=\joinrel=\joinrel=\joinrel=}}\int\frac{d\theta}{\sqrt{5}\sin\theta}\\
	&=-\frac{1}{\sqrt{5}}\csc\theta\cot\theta+C
	\end{align*}

\item%15
	\begin{align*}
	\int_0^ax^2\sqrt{a^2-x^2}\ dx&\overset{x=a\sin\theta}{\underset{dx=a\cos\theta\ d\theta}{=\joinrel=\joinrel=\joinrel=\joinrel=\joinrel=\joinrel=\joinrel=}}a^4\int_0^a\sin^2\theta\cos^2\theta\ d\theta\\
	&=a^4\int_0^a(1-\cos(2\theta))(1+\cos(2\theta))\ d\theta\\
	&=a^4\int_0^a1-\cos^2(2\theta)\ d\theta\\
	&=-a^4\int_0^a\cos(4\theta)\ d\theta\\
	&=-\frac{a^4}{4}\sin(4\theta)\Big|_0^a\\
	&=-\frac{a^4}{4}\sin(4a)
	\end{align*}

\item%16
	\begin{align*}
	\int_{\sqrt{2}/3}^{2/3}\frac{dx}{x^5\sqrt{9x^2-1}}&\overset{u=3x}{\underset{du=3\ dx}{=\joinrel=\joinrel=\joinrel=\joinrel=}}3^4\int_{\sqrt{2}}^2\frac{1}{u^5\sqrt{u^2-1}}\ du\\
	&\overset{u=\sec\theta}{\underset{du=\sec\theta\tan\theta\ d\theta}{=\joinrel=\joinrel=\joinrel=\joinrel=\joinrel=\joinrel=\joinrel=\joinrel=\joinrel=}}3^4\int_\frac{\pi}{4}^\frac{\pi}{3}\frac{\sec\theta\tan\theta}{\sec^5\theta\tan\theta}\ d\theta\\
	&=\int_\frac{\pi}{4}^\frac{\pi}{3}\cos^4\theta\ d\theta\\
	&=\int_\frac{\pi}{4}^\frac{\pi}{3}\left(\frac{1+\cos(2\theta)}{2}\right)^2\ d\theta\\
	&=\int_\frac{\pi}{4}^\frac{\pi}{3}\frac{1}{4}+\frac{1}{2}\cos(2\theta)+\frac{1}{4}\cos^2(2\theta)\ d\theta\\
	&=\int_\frac{\pi}{4}^\frac{\pi}{3}\frac{3}{8}+\frac{1}{2}\cos(2\theta)+\frac{1}{8}\cos(4\theta)\ d\theta\\
	&=\frac{3}{8}\theta+\frac{1}{4}\sin(2\theta)+\frac{1}{32}\sin(4\theta)\Big|_\frac{\pi}{4}^\frac{\pi}{3}\\
	&=\left[\frac{\pi}{8}+\frac{\sqrt{3}}{8}-\frac{\sqrt{3}}{64}\right]-\left[\frac{3\pi}{32}\right]
	\end{align*}

\color{red}\item[\refstepcounter{enumi}\fbox{\number\value{enumi}.}]\color{black}%17
	\begin{align*}
	\int\frac{x}{\sqrt{x^2-7}}\ dx&\overset{x=\sqrt{7}\sec\theta}{\underset{dx=\sqrt{7}\sec\theta\tan\theta\ d\theta}{=\joinrel=\joinrel=\joinrel=\joinrel=\joinrel=\joinrel=\joinrel=\joinrel=\joinrel=\joinrel=\joinrel=}}\int\frac{\sqrt{7}\sec\theta}{\sqrt{7}\tan\theta}\cdot\sqrt{7}\sec\theta\tan\theta\ d\theta\\
	&=\sqrt{7}\int\sec^2\theta\ d\theta\\
	&=\sqrt{7}\tan\theta+C
	\end{align*}

\item%18
	\begin{align*}
	\int\frac{dx}{[(ax)^2-b^2]^{3/2}}&=\int\frac{dx}{\left(\sqrt{a^2(x^2-b^2/a^2)}\right)^3}\\
	&=\int\frac{dx}{\left(a\sqrt{(x^2-b^2/a^2)}\right)^3}\\
	&\overset{x=\frac{b}{a}\sec\theta}{\underset{dx=\frac{b}{a}\sec\theta\tan\theta\ d\theta}{=\joinrel=\joinrel=\joinrel=\joinrel=\joinrel=\joinrel=\joinrel=\joinrel=\joinrel=\joinrel=}}\int\frac{\frac{b}{a}\sec\theta\tan\theta\ d\theta}{a^3\cdot\frac{b^3}{a^3}\tan^3\theta}\\
	&=\frac{1}{ab^2}\int\sec\theta\cot^2\theta\ d\theta\\
	&=\frac{1}{ab^2}\int\frac{\cos\theta}{\sin^2\theta}\ d\theta\\
	&\overset{u=\sin\theta}{\underset{du=\cos\theta\ d\theta}{=\joinrel=\joinrel=\joinrel=\joinrel=\joinrel=\joinrel=}}
	\end{align*}

\item%19
	\begin{align*}
	\int\frac{\sqrt{1+x^2}}{x}\ dx&\overset{x=\tan\theta}{\underset{dx=\sec^2\theta\ d\theta}{=\joinrel=\joinrel=\joinrel=\joinrel=\joinrel=\joinrel=\joinrel=}}\int\frac{\sec\theta}{\tan\theta}\cdot\sec^2\theta\ d\theta\\
	&=\int\csc\theta\sec^2\theta\ d\theta\\
	&=\int\csc\theta+\tan^2\theta\csc\theta\\
	&=\int\csc\theta+\tan\theta\sec\theta\\
	&=\int\frac{\csc^2\theta+\csc\theta\cot\theta}{\csc\theta+\cot\theta}+\sec\theta\tan\theta\ d\theta\\
	&\overset{u=\csc\theta+\cot\theta}{\underset{du=-\csc\theta\cot\theta-\csc^2\theta\ d\theta}{=\joinrel=\joinrel=\joinrel=\joinrel=\joinrel=\joinrel=\joinrel=\joinrel=\joinrel=\joinrel=\joinrel=\joinrel=\joinrel=\joinrel=\joinrel=}}-\int\frac{du}{u}+\int\sec\theta\tan\theta\ d\theta\\
	&=\ln|\csc\theta+\cot\theta|+\sec\theta+C
	\end{align*}

\item%20
	\begin{align*}
	\int\frac{t}{\sqrt{25-t^2}}\ dt&\overset{t=5\sin\theta}{\underset{dt=5\cos\theta\ d\theta}{=\joinrel=\joinrel=\joinrel=\joinrel=\joinrel=\joinrel=\joinrel=}}\int\frac{5\sin\theta}{5\cos\theta}\cdot5\cos\theta\ d\theta\\
	&=-5\cos\theta+C
	\end{align*}

\item%21
	\begin{align*}
	\int_0^{0.6}\frac{x^2}{\sqrt{9-25x^2}}\ dx&=\int_0^\frac{3}{5}\frac{x^2}{5\sqrt{\frac{9}{25}-x^2}}\ dx\\
	&\overset{x=\frac{3}{5}\sin t}{\underset{dx=\frac{3}{5}\cos t\ dt}{=\joinrel=\joinrel=\joinrel=\joinrel=\joinrel=\joinrel=\joinrel=}}\int_0^\frac{\pi}{2}\frac{\frac{3^2}{5^2}\sin^2t}{5\cdot\frac{3}{5}\cos t}\cdot\frac{3}{5}\cos t\ dt\\
	&=\frac{3^2}{5^3}\int_0^\frac{\pi}{2}\sin^2t\ dt\\
	&=\frac{3^2}{2\cdot5^3}\int_0^\frac{\pi}{2}1-\cos(2t)\ dt\\
	&=\frac{3^2}{2\cdot5^3}[t-\frac{1}{2}\sin(2t)]_0^\frac{\pi}{2}\\
	&=\frac{3^2}{2^2\cdot5^3}\pi
	\end{align*}

\color{red}\item[\refstepcounter{enumi}\fbox{\number\value{enumi}.}]\color{black}%22

\item%23
	\begin{align*}
	\int\sqrt{5+4x-x^2}\ dx&=\int\sqrt{9-(x-2)^2}\ dx\\
	&\overset{u=x-2}{\underset{du=\ dx}{=\joinrel=\joinrel=\joinrel=\joinrel=}}\int\sqrt{9-u^2}\ du\\
	&\overset{u=3\sin t}{\underset{du=3\cos t\ dt}{=\joinrel=\joinrel=\joinrel=\joinrel=\joinrel=\joinrel=\joinrel=}}3\int\cos u\ du\\
	&=3\sin u+C
	\end{align*}

\item%24
	\begin{align*}
	\int\frac{dt}{\sqrt{t^2-6t+13}}&=\int\frac{dt}{\sqrt{(t-3)^2+4}}\\
	&\overset{u=t-3}{\underset{du=\ dt}{=\joinrel=\joinrel=\joinrel=\joinrel=}}\int\frac{du}{\sqrt{u^2+4}}\\
	&\overset{u=2\tan t}{\underset{du=2\sec^2 t\ dt}{=\joinrel=\joinrel=\joinrel=\joinrel=\joinrel=\joinrel=\joinrel=}}\int\sec t\ dt\\
	&=\int\frac{\sec^2t+\sec t\tan t}{\sec t+\tan t}\ dt\\
	&\overset{w=\sec t+\tan t}{\underset{dw=\sec t\tan t+\sec^2t\ dt}{=\joinrel=\joinrel=\joinrel=\joinrel=\joinrel=\joinrel=\joinrel=\joinrel=\joinrel=\joinrel=\joinrel=\joinrel=\joinrel=}}\ln|\sec t+\tan t|+C
	\end{align*}

\item%25
	\begin{align*}
	\int\frac{x}{\sqrt{x^2+x+1}}\ dx&=\scaleint{10ex}\frac{x}{\sqrt{\left(x+\frac{1}{2}\right)^2+\frac{3}{4}}}\ dx\\
	&\overset{x=\frac{\sqrt{3}}{2}\tan\theta-\frac{1}{2}}{\underset{dx=\frac{\sqrt{3}}{2}\sec^2\theta\ d\theta}{=\joinrel=\joinrel=\joinrel=\joinrel=\joinrel=\joinrel=\joinrel=\joinrel=\joinrel=\joinrel=}}
	\end{align*}

\item%26
	\begin{align*}
	\scaleint{7ex}\frac{x^2}{(3+4x-4x^2)^{3/2}}\ dx&=\scaleint{9ex}\frac{x^2}{\left(\sqrt{-4[x^2-4x]+3}\right)^3}\\
	&=\scaleint{9ex}\frac{x^2}{\left(\sqrt{19-4(x-2)^2}\right)^3}\\
	&=\frac{1}{8}\scaleint{11ex}\frac{x^2}{\left(\sqrt{\frac{19}{4}-(x-2)^2}\right)^3}\\
	&\overset{x=\frac{\sqrt{19}}{2}\sin\theta+2}{\underset{dx=\frac{\sqrt{19}}{2}\cos\theta+\frac{1}{2}\theta\ d\theta}{=\joinrel=\joinrel=\joinrel=\joinrel=\joinrel=\joinrel=\joinrel=\joinrel=\joinrel=}}
	\end{align*}
\end{enumerate}
\end{document}