\documentclass[a4]{article}

%other packages
\usepackage[a4paper, total={7.5in, 10.5in}]{geometry}
\usepackage{longtable}
\usepackage{wrapfig}
\setlength\parindent{0pt}
\usepackage{enumitem}
\usepackage[table]{xcolor}

%maths
\usepackage{mathtools}
\usepackage{amsmath}
\usepackage{amssymb}
\usepackage{amsfonts}
\usepackage{autobreak}

%tikzpicture
\usepackage{tikz}
\usepackage{scalerel}
\usepackage{pict2e}
\usepackage{tkz-euclide}
\usetikzlibrary{calc}
\usetikzlibrary{patterns,arrows.meta}
\usetikzlibrary{shadows}
\usetikzlibrary{external}

%pgfplots
\usepackage{pgfplots}
\pgfplotsset{compat=newest}
\usepgfplotslibrary{statistics}
\usepgfplotslibrary{fillbetween}

\begin{document}
\begin{enumerate}[label={\bf{}\arabic*}.]
\item%1
	$\int x^2\ln x\ dx\overset{u=\ln x,\ du=\frac{1}{x}\ dx}{\underset{dv=x^2\ dx,\ v=\frac{1}{3}x^3}{=\joinrel=\joinrel=\joinrel=\joinrel=\joinrel=\joinrel=\joinrel=\joinrel=\joinrel=\joinrel=\joinrel=}}\ln x\frac{1}{3}x^3-\frac{1}{3}\int x^2\ dx=\frac{1}{3}x^3\ln x-\frac{1}{9}x^3+C$

\item%2
	$\int\theta\cos\theta\ d\theta\overset{u=\theta,\ du=d\theta}{\underset{dv=\cos\theta\ d\theta,\ v=\sin\theta}{=\joinrel=\joinrel=\joinrel=\joinrel=\joinrel=\joinrel=\joinrel=\joinrel=\joinrel=\joinrel=\joinrel=\joinrel=\joinrel=}}
\theta\sin\theta-\int\sin\theta\ d\theta=\theta\sin\theta+\cos\theta+C$

\item%3
	$\int x\cos 5x\ dx\underset{dv=\cos5x\ dx\Rightarrow v=\frac{1}{5}\sin5x}{\overset{u=x\Rightarrow du=dx}{=\joinrel=\joinrel=\joinrel=\joinrel=\joinrel=\joinrel=\joinrel=\joinrel=\joinrel=\joinrel=\joinrel=\joinrel=\joinrel=\joinrel=}}\frac{x}{5}\sin5x-\frac{1}{5}\int\sin5x\ dx=\frac{x}{5}\sin5x+\frac{1}{25}\cos5x+C$

\item%4
	$\int xe^{-x}\ dx\overset{u=x\Rightarrow du=dx}{\underset{dv=e^{-x}\Rightarrow v=-e^{-x}}{=\joinrel=\joinrel=\joinrel=\joinrel=\joinrel=\joinrel=\joinrel=\joinrel=\joinrel=\joinrel=}}-xe^{-x}-\int e^{-x}\ dx=-xe^{-x}-e^{-x}+C$

\item%5
	$\int re^{r/2}\ dr\overset{u=r,\ du=dv}{\underset{dv=e^{\frac{1}{2}r},\ v=2e^{\frac{1}{2}r}}{=\joinrel=\joinrel=\joinrel=\joinrel=\joinrel=\joinrel=\joinrel=\joinrel=\joinrel=\joinrel=}}2re^{\frac{r}{2}}-2\int e^\frac{r}{2}\ dr=2re^\frac{r}{2}-4e^\frac{r}{2}+C$

\item%6
	$\int t\sin2t\ dt\overset{u=t,\ du=dt}{\underset{dv=\sin2t\ dt,\ v=-\frac{1}{2}\cos2t}{\joinrel=\joinrel=\joinrel=\joinrel=\joinrel=\joinrel=\joinrel=\joinrel=\joinrel=\joinrel=\joinrel=\joinrel=\joinrel=\joinrel=\joinrel=}}-\frac{t}{2}\cos2t+\frac{1}{2}\int\cos2t\ dt=-\frac{t}{2}\cos2t+\frac{1}{4}\sin2t+C$

\item%7
	$\int x^2\sin\pi x\ dx\overset{u=x^2,\ du=2x\ dx}{\underset{dv=\sin\pi x,\ v=-\frac{1}{\pi}\cos\pi x}{=\joinrel=\joinrel=\joinrel=\joinrel=\joinrel=\joinrel=\joinrel=\joinrel=\joinrel=\joinrel=\joinrel=\joinrel=\joinrel=\joinrel=}}-\frac{x^2}{\pi}\cos\pi x+\frac{2}{\pi}\int x\cos\pi x\overset{u=x,\ du=dx}{\underset{dv=\cos\pi x,\ v=\frac{1}{\pi}\sin\pi x}{=\joinrel=\joinrel=\joinrel=\joinrel=\joinrel=\joinrel=\joinrel=\joinrel=\joinrel=\joinrel=\joinrel=\joinrel=}}\frac{x^2}{\pi}\cos\pi x+\frac{x}{\pi}\sin\pi x+\frac{1}{\pi^2}\cos\pi x+C$

\item%8
	$\int x^2\cos mx\ dx\overset{u=x^2,\ du=2x\ dx}{\underset{dv=\cos mx\ dx,\ v=\frac{1}{m}\sin mx}{=\joinrel=\joinrel=\joinrel=\joinrel=\joinrel=\joinrel=\joinrel=\joinrel=\joinrel=\joinrel=\joinrel=\joinrel=\joinrel=\joinrel=\joinrel=}}\frac{x^2}{m}\sin mx-\frac{2}{m}\int x\sin mx\ dx\overset{u=x,\ du=dx}{\underset{dv=\sin mx\ dx,\ v=-\frac{1}{m}\cos mx}{=\joinrel=\joinrel=\joinrel=\joinrel=\joinrel=\joinrel=\joinrel=\joinrel=\joinrel=\joinrel=\joinrel=\joinrel=\joinrel=\joinrel=\joinrel=\joinrel=\joinrel=}}\frac{x^2}{m}\sin mx+\frac{2x}{m^2}\cos mx+\frac{2}{m^2}\int\cos mx\ dx=\frac{x^2}{m}\sin mx+\frac{2x}{m^2}\cos mx+\frac{2}{m^3}\sin mx+C$

\item%9
	$\int\ln(2x+1)\ dx\overset{u=\ln(2x+1),\ du=\frac{2}{2x+1}\ dx}{\underset{dv=dx,\ v=x}{=\joinrel=\joinrel=\joinrel=\joinrel=\joinrel=\joinrel=\joinrel=\joinrel=\joinrel=\joinrel=\joinrel=\joinrel=\joinrel=\joinrel=\joinrel=}}x\ln(2x+1)-\int\frac{2x}{2x+1}\ dx\overset{u=2x+1,\ du=2\ dx}{\underset{x=\frac{u-1}{2}}{=\joinrel=\joinrel=\joinrel=\joinrel=\joinrel=\joinrel=\joinrel=\joinrel=\joinrel=\joinrel=}}x\ln(2x+1)-\int\frac{\frac{u-1}{2}}{u}\ du=x\ln(2x+1)-\frac{1}{2}(2x+1)-\frac{1}{2}\ln(2x+1)+C$

\item%10
	$\int\arcsin x\ dx\overset{u=\arcsin x,\ du=\frac{1}{\sqrt{1-x^2}}\ dx}{\underset{dv=dx,\ v=x }{=\joinrel=\joinrel=\joinrel=\joinrel=\joinrel=\joinrel=\joinrel=\joinrel=\joinrel=\joinrel=\joinrel=\joinrel=\joinrel=\joinrel=\joinrel=}}x\arcsin x+\frac{1}{2}\int\frac{-2x}{\sqrt{1-x^2}}\ dx\overset{u=1-x^2,\ du=-2x\ dx}{=\joinrel=\joinrel=\joinrel=\joinrel=\joinrel=\joinrel=\joinrel=\joinrel=\joinrel=\joinrel=\joinrel=\joinrel=}x\arcsin x+\frac{1}{2}\int u^{-1/2}\ du=x\arcsin x-\frac{1}{4}u^{-3/2}=x\arcsin x-\frac{1}{4}(1-x^2)^{-3/2}+C$

\item%11
	$\int\arctan4t\ dt\overset{u=\arctan4t,\ du=\frac{4}{16t^2+1}\ dt}{\underset{dv=dt,\ v=t}{=\joinrel=\joinrel=\joinrel=\joinrel=\joinrel=\joinrel=\joinrel=\joinrel=\joinrel=\joinrel=\joinrel=\joinrel=\joinrel=\joinrel=\joinrel=\joinrel=}}t\arctan4t-\frac{1}{8}\int\frac{32t}{16t^2+1}\ dt\overset{u=16t^2,\ du=32t\ dt}{=\joinrel=\joinrel=\joinrel=\joinrel=\joinrel=\joinrel=\joinrel=\joinrel=\joinrel=\joinrel=\joinrel=}t\arctan4t-\frac{1}{8}\ln|16t^2+1|+C$

\item%12
	$\int p^5\ln p\ dp\overset{u=\ln p,\ du=p^{-1}\ dp}{\underset{dv=p^5\ dp,\ v=\frac{1}{6}p^6}{=\joinrel=\joinrel=\joinrel=\joinrel=\joinrel=\joinrel=\joinrel=\joinrel=\joinrel=\joinrel=\joinrel=}}\frac{p^6}{6}\ln p-\frac{1}{6}\int p^5\ dp=\frac{p^6}{6}\ln p-\frac{p^6}{36}+C$

\item%13
	$\int t\sec^22t\ dt\overset{u=t,\ du=dt}{\underset{dv=\sec^22t\ dt,\ v=\frac{1}{2}\tan2t}{=\joinrel=\joinrel=\joinrel=\joinrel=\joinrel=\joinrel=\joinrel=\joinrel=\joinrel=\joinrel=\joinrel=\joinrel=\joinrel=\joinrel=}}\frac{t}{2}\tan2t-\frac{1}{4}\int2\tan2t\ dt=\frac{t}{2}\tan2t-\ln|\sec2t|+C$

\item%14
	$\int s2^s\ ds\overset{u=s,\ du=ds}{\underset{dv=2^s\ ds,\ v=\frac{2^s}{\ln2}}{=\joinrel=\joinrel=\joinrel=\joinrel=\joinrel=\joinrel=\joinrel=\joinrel=\joinrel=\joinrel=}}\frac{s2^s}{\ln2}-\frac{1}{\ln2}\int2^s\ ds=\frac{s2^s}{\ln2}-\frac{1}{(\ln2)^2}2^s+C$

\item%15
	$\int(\ln x)^2\ dx\overset{u=(\ln x)^2,\ du=\frac{2\ln x}{x}\ dx}{\underset{dv=dx,\ v=x}{=\joinrel=\joinrel=\joinrel=\joinrel=\joinrel=\joinrel=\joinrel=\joinrel=\joinrel=\joinrel=\joinrel=\joinrel=\joinrel=}}x(\ln x)^2-2\int\ln x\ dx\overset{u=\ln x,\ du=\frac{1}{x}\ dx}{\underset{dv=dx,\ v=x}{=\joinrel=\joinrel=\joinrel=\joinrel=\joinrel=\joinrel=\joinrel=\joinrel=\joinrel=}}x(\ln x)^2-2x\ln x-2x+C$

\item%16
	$\int t\sinh mt\ dt\overset{u=t,\ du=dt}{\underset{dv=\sinh mt\ dt,\ v=\frac{1}{m}\cosh mt}{=\joinrel=\joinrel=\joinrel=\joinrel=\joinrel=\joinrel=\joinrel=\joinrel=\joinrel=\joinrel=\joinrel=\joinrel=\joinrel=\joinrel=\joinrel=\joinrel=}}\frac{t}{m}\cosh mt-\frac{1}{m^2}\sinh mt+C$

\item%17
	$\int e^{2\theta}\sin3\theta\ d\theta\overset{u=\sin3\theta,\ du=3\cos3\theta\ d\theta}{\underset{dv=e^{2\theta}\ d\theta,\ v=\frac{1}{2}e^{2\theta}}{=\joinrel=\joinrel=\joinrel=\joinrel=\joinrel=\joinrel=\joinrel=\joinrel=\joinrel=\joinrel=\joinrel=\joinrel=\joinrel=\joinrel=}}\frac{1}{2}e^{2\theta}\sin3\theta-\frac{3}{2}\int e^{2\theta}\cos3\theta\ d\theta\overset{u=\cos3\theta,\ du=-3\sin3\theta\ d\theta}{\underset{dv=e^{2\theta}\ d\theta,\ v=\frac{1}{2}e^{2\theta}}{=\joinrel=\joinrel=\joinrel=\joinrel=\joinrel=\joinrel=\joinrel=\joinrel=\joinrel=\joinrel=\joinrel=\joinrel=\joinrel=\joinrel=\joinrel=}}\frac{1}{2}e^{2\theta}\sin3\theta-\frac{3}{4}e^{2\theta}\cos3\theta+\frac{9}{4}\int e^{2\theta}\sin3\theta\ d\theta\Rightarrow\int e^{2\theta}\sin3\theta\ d\theta=-\frac{2}{5}e^{2\theta}\sin3\theta+\frac{3}{5}e^{2\theta}\cos3\theta+C$

\item%18
	$\int e^{-\theta}\cos2\theta\ d\theta\overset{u=e^{-\theta},\ du=-e^{-\theta}\ d\theta}{\underset{dv=\cos2\theta\ d\theta,\ v=\frac{1}{2}\sin2\theta}{=\joinrel=\joinrel=\joinrel=\joinrel=\joinrel=\joinrel=\joinrel=\joinrel=\joinrel=\joinrel=\joinrel=\joinrel=\joinrel=\joinrel=}}\frac{1}{2}e^{-\theta}\sin2\theta+\frac{1}{2}\int e^{-\theta}\sin2\theta\ d\theta\overset{u=e^{-\theta},\ du=-e^{-\theta}\ d\theta}{\underset{dv=\sin2\theta\ d\theta,\ v=-\frac{1}{2}\cos2\theta}{=\joinrel=\joinrel=\joinrel=\joinrel=\joinrel=\joinrel=\joinrel=\joinrel=\joinrel=\joinrel=\joinrel=\joinrel=\joinrel=\joinrel=\joinrel=}}\frac{1}{2}e^{-\theta}\sin2\theta-\frac{1}{4}e^{-\theta}\cos2\theta-\frac{1}{2}\int e^{-\theta}\cos2\theta=\frac{2}{3}e^{-\theta}\sin2\theta+C$

\item%19
	$\int_0^\pi t\sin3t\ dt\overset{u=t,\ du=dt}{\underset{dv=\sin3t\ dt,\ v=-\frac{1}{3}\cos3t}{=\joinrel=\joinrel=\joinrel=\joinrel=\joinrel=\joinrel=\joinrel=\joinrel=\joinrel=\joinrel=\joinrel=\joinrel=\joinrel=\joinrel=\joinrel=}}-\frac{1}{3}t\cos3t|_0^\pi+\frac{1}{3}\int_0^\pi\cos3t\ dt=\frac{\pi}{3}+\frac{1}{9}\sin3t|_0^\pi=\frac{pi}{3}$

\item%20
	$\int_0^1(x^2+1)e^{-x}\ dx\overset{u=x^2+1,\ du=2x\ dx}{\underset{dv=e^{-x}\ dx,\ v=-e^{-x}}{=\joinrel=\joinrel=\joinrel=\joinrel=\joinrel=\joinrel=\joinrel=\joinrel=\joinrel=\joinrel=\joinrel=\joinrel=}}-(x^2+1)e^{-x}|_0^1+2\int xe^{-x}\ dx\overset{u=x,\ du=dx}{\underset{dv=e^{-x}\ dx,\ v=-e^{-x}}{=\joinrel=\joinrel=\joinrel=\joinrel=\joinrel=\joinrel=\joinrel=\joinrel=\joinrel=\joinrel=\joinrel=\joinrel=\joinrel=}}-(x^2+1)e^{-x}|_0^1-2xe^{-x}-2e^{-x}|_0^1=-(x^2+x+3)e^{-x}|_0^1=-\frac{5}{e}+3$

\item%21
	$\int_0^1t\cosh t\ dt\overset{u=t,\ du=dt}{\underset{dv=\cosh t\ dt,\ v=\sinh t}{=\joinrel=\joinrel=\joinrel=\joinrel=\joinrel=\joinrel=\joinrel=\joinrel=\joinrel=\joinrel=\joinrel=\joinrel=}}t\sinh t|_0^1-\int_0^1\sinh t\ dt=t\sinh t-\cosh t|_0^1=\frac{e-e^{-1}}{2}-(\frac{e+e^{-1}}{2}-1)=-\frac{1}{e}+1$

\item%22
	\begin{align*}
	\int_4^9\frac{\ln y}{\sqrt{y}}\ dy&\overset{u=\ln y,\ du=\frac{1}{y}\ dy}{\underset{dv=y^{-\frac{1}{2}},\ v=2\sqrt{y}}{=\joinrel=\joinrel=\joinrel=\joinrel=\joinrel=\joinrel=\joinrel=\joinrel=\joinrel=\joinrel=}}\left.\ln y\cdot2\sqrt{y}\right|_4^9-\int_4^92\sqrt{y}\cdot\frac{1}{y}\ dy\\
	&=6\ln9-4\ln4-2\int_4^9y^{-1/2}\ dy\\
	&=6\ln9-4\ln4-4\sqrt{y}|_4^9\\
	&=6\ln9-4\ln4-4
	\end{align*}

\item%23
	\begin{align*}
	\int_1^2\frac{\ln x}{x^2}\ dx&\overset{u=\ln x,\ du=\frac{1}{x}\ dx}{\underset{dv=\frac{1}{x^2}\ dx,\ v=-\frac{1}{x}}{=\joinrel=\joinrel=\joinrel=\joinrel=\joinrel=\joinrel=\joinrel=\joinrel=\joinrel=\joinrel=}}-\frac{1}{x}\ln x\Big|_1^2+\int\frac{1}{x^2}\ dx\\
	&=-\frac{1}{x}(\ln x+1)\Big|_1^2\\
	&=-\frac{1}{2}(\ln2+1)+1
	\end{align*}

\item%24
	\begin{align*}
	\int_0^\pi x^3\cos x\ dx&\overset{u=x^3,\ du=3x^2\ dx}{\underset{dv=\cos x\ dx,\ v=\sin x}{=\joinrel=\joinrel=\joinrel=\joinrel=\joinrel=\joinrel=\joinrel=\joinrel=\joinrel=\joinrel=\joinrel=\joinrel=}}x^3\sin x\Big|_0^\pi-\int_0^\pi3x^2\sin x\ dx\\
	&\overset{u=x^2,\ du=2x\ dx}{\underset{dv=\sin x\ dx,\ v=-\cos x}{=\joinrel=\joinrel=\joinrel=\joinrel=\joinrel=\joinrel=\joinrel=\joinrel=\joinrel=\joinrel=\joinrel=\joinrel=\joinrel=}}x^3\sin x\Big|_0^\pi-3\left[-x^2\cos x\Big|_0^\pi+2\int_0^\pi x\cos x\ dx\right]\\
	&\overset{u=x,\ du=dx}{\underset{dv=\cos x,\ v=\sin x}{=\joinrel=\joinrel=\joinrel=\joinrel=\joinrel=\joinrel=\joinrel=\joinrel=\joinrel=}}x^3\sin x\Big|_0^\pi-3\left[-x^2\cos x\Big|_0^\pi+2\left[x\sin x\Big|_0^\pi-\int_0^\pi\sin x\ dx\right]\right]\\
	&=x^3\sin x\Big|_0^\pi-3\left[-x^2\cos x\Big|_0^\pi+2\left[x\sin x\Big|_0^\pi+\cos x\Big|_0^\pi\right]\right]\\
	&=-3\pi^2+12
	\end{align*}

\item%25
	\begin{align*}
	\int_0^1\frac{y}{e^{2y}}\ dy&\overset{u=y,\ du=\ dy}{\underset{dv=e^{-2y},\ v=-\frac{1}{2}e^{-2y}}{=\joinrel=\joinrel=\joinrel=\joinrel=\joinrel=\joinrel=\joinrel=\joinrel=\joinrel=\joinrel=\joinrel=\joinrel=}}\frac{-y}{2}e^{-2y}\Big|_0^1+\frac{1}{2}\int_0^1e^{-2y}\ dy\\
	&=\frac{-2y-1}{4}e^{-2y}\Big|_0^1\\
	&=[(\frac{-3}{4}e^{-2})-(\frac{-1}{4})]
	\end{align*}

\item%26
	\begin{align*}
	\int_1^{\sqrt{3}}\arctan(1/x)\ dx\overset{u=\arctan(1/x),\ du=\frac{-1}{x^2+1}}{\underset{dv=1,\ v=x}{=\joinrel=\joinrel=\joinrel=\joinrel=\joinrel=\joinrel=\joinrel=\joinrel=\joinrel=\joinrel=\joinrel=\joinrel=\joinrel=\joinrel=\joinrel=}}
	\end{align*}



\end{enumerate}
\end{document}